stdlib/ptr/output/ptr/proofs/proof_const_ptr_wrapping_add.v
@@ -1,0 +1,45 @@
+From caesium Require Import lang notation.
+From refinedrust Require Import typing shims.
+From stdlib.ptr.ptr.generated Require Import generated_code_ptr generated_specs_ptr generated_template_const_ptr_wrapping_add.
+
+Set Default Proof Using "Type".
+
+Section proof.
+Context `{RRGS : !refinedrustGS Σ}.
+
+Lemma const_ptr_wrapping_add_proof (π : thread_id) :
+  const_ptr_wrapping_add_lemma π.
+Proof.
+  const_ptr_wrapping_add_prelude.
+
+  repeat liRStep; liShow.
+  liFromSyntax.
+  rewrite /typed_bin_op/typed_val_expr.
+  iIntros "Hv1 Hv2" (Φ) "#CTX #HE HL Hcont".
+  rewrite {1}/ty_own_val /=. iDestruct "Hv1" as %[Hv1 Hsz1].
+  rewrite {1}/ty_own_val /=. iDestruct "Hv2" as "->".
+  iRename select (credit_store _ _) into "Hstore".
+  iPoseProof (credit_store_borrow_receipt with "Hstore") as "(Hat & Hatcl)".
+  iDestruct "CTX" as "(LFT & TIME & LLCTX)".
+  iMod (persistent_time_receipt_0) as "Hp".
+  iApply (wp_ptr_wrapping_offset_credits with "TIME Hat Hp").
+  { done. }
+  { apply val_to_of_loc. }
+  { done. }
+  iNext. simpl. iEval (rewrite additive_time_receipt_succ). iIntros "Hcred [Hat Hat']".
+  iPoseProof ("Hatcl" with "Hat'") as "Hstore".
+  iPoseProof (credit_store_donate with "Hstore Hcred") as "Hstore".
+  iPoseProof (credit_store_donate_atime with "Hstore Hat") as "Hstore".
+  iApply ("Hcont" $! _ π _ _ (alias_ptr_t) with "HL").
+  { rewrite /ty_own_val /=. done. }
+
+  repeat liRStep; liShow.
+
+  all: print_remaining_goal.
+  Unshelve. all: sidecond_solver.
+  Unshelve. all: sidecond_hammer.
+  { rewrite /WrappingOffsetLocSt.
+    simplify_layout_goal. done. }
+  Unshelve. all: print_remaining_sidecond.
+Qed.
+End proof.
